more on systemfwithnat

Examples/SystemFWithNat/Term.lean
@@ -18,7 +18,7 @@ inductive Term where
 | app : Term -> Term -> Term
 | lam (A : Ty) (t : Term) : Term -- binds Term in t
 | tapp : Term -> Ty -> Term
-| tlam (t : Term) : Term -- binds Ty in t (does it make sense to allow a user to give a name sinstead of a position?)
+| tlam (t : Term) : Term -- binds Ty in t (does it make sense to allow a user to give a name instead of a position?)
 | zero : Term
 | succ : Term -> Term
 | nrec (motive : Ty) (z : Term) (s : Term) (n : Term) : Term -- binds 2 Term's in s
@@ -36,25 +36,28 @@ inductive Term where
 
 #leansubst generate Ty, Term
 
+-- Ty --
 #print Ty.rmap
 #print Ty.rmap._f
 
+#print Ty.rmap_var
+#print Ty.rmap_arrow
+#print Ty.rmap_all
+#print Ty.rmap_nat
+
+-- Term --
 #print Term.rmap
 #print Term.rmap._f
 
-/-
+#print Term.rmap_var
+#print Term.rmap_app
+#print Term.rmap_lam
+#print Term.rmap_tapp
+#print Term.rmap_tlam
+#print Term.rmap_zero
+#print Term.rmap_succ
+#print Term.rmap_nrec
 
-#leansubst var Ty.var
-#leansubst bind 1 of Ty in Ty.all at pos 0
-
-#leansubst var Term.var
-#leansubst bind 1 of Term in Term.lam at pos 1
-#leansubst bind 1 of Ty in Term.tlam at pos 0
-#leansubst bind 2 of Term in Term.nrec at pos 2
-
-#leansubst generate Ty, Term
-
--/
 
 ----------------------------------------------------------------------------------------------------
 -- Ty Renaming & Substitution
@@ -62,58 +65,75 @@ inductive Term where
 
 -- This is just STLC with some constants
 
-instance : RenMap Ty [Ty] where
-  rmap := sorry
+-- instance : RenMap Ty [Ty] where
+  -- rmap := sorry
 
-instance : SubstMap Ty [Ty] where
-  smap := sorry
+-- instance : SubstMap Ty [Ty] where
+  -- smap := sorry
 
 ----------------------------------------------------------------------------------------------------
 -- Term Renaming & Substitution
 ----------------------------------------------------------------------------------------------------
 
-@[coe]
-def Term.from_action : Action Term -> Term
-| re y => var y
-| su t => t
+-- @[coe]
+-- def Term.from_action : Action Term -> Term
+-- | re y => var y
+-- | su t => t
 
-@[simp, grind =]
-theorem Term.from_action_id {n} : from_action (𝐬0.act n) = var n := by
-  simp [from_action]
+-- @[simp, grind =]
+-- theorem Term.from_action_id {n} : from_action (𝐬0.act n) = var n := by
+--   simp [from_action]
 
-@[simp, grind =]
-theorem Term.from_action_succ {n} : from_action (𝐬1.act n) = var (n + 1) := by
-  simp [from_action]
+-- @[simp, grind =]
+-- theorem Term.from_action_succ {n} : from_action (𝐬1.act n) = var (n + 1) := by
+--   simp [from_action]
 
-@[simp, grind =]
-theorem Term.from_action_re {n} : from_action (re n) = var n := by simp [from_action]
+-- @[simp, grind =]
+-- theorem Term.from_action_re {n} : from_action (re n) = var n := by simp [from_action]
 
-@[simp, grind =]
-theorem Term.from_action_su {t} : from_action (su t) = t := by simp [from_action]
+-- @[simp, grind =]
+-- theorem Term.from_action_su {t} : from_action (su t) = t := by simp [from_action]
 
-instance : Coe (Action Term) Term where
-  coe := Term.from_action
+-- instance : Coe (Action Term) Term where
+--   coe := Term.from_action
 
 -- Defining the rmap/smap using the Tuple form might make more sense for a macro, dunno
 @[simp]
-def Term.rmap (r : RenVec [Term, Ty]) : Term -> Term
+def Term.rmap' (r : RenVec [Term, Ty]) : Term -> Term
 | var x => var (r.1.act x)
-| app t1 t2 => app (t1.rmap r) (t2.rmap r)
-| lam A t => lam A⟨r.2.1⟩ (rmap (r.lift [1, 0]) t)
-| tapp t A => tapp (t.rmap r) A⟨r.2.1⟩
-| tlam t => tlam (t.rmap $ r.lift [0, 1])
+| app t1 t2 => app (t1.rmap' r) (t2.rmap' r)
+| lam A t => lam A⟨r.2.1⟩ (rmap' (r.lift [1, 0]) t)
+| tapp t A => tapp (t.rmap' r) A⟨r.2.1⟩
+| tlam t => tlam (t.rmap' $ r.lift [0, 1])
 | zero => zero
-| succ t => succ (t.rmap r)
-| nrec motive z s n => nrec motive⟨r.2.1⟩ (z.rmap r) (s.rmap $ r.lift [2, 0]) (n.rmap r)
+| succ t => succ (t.rmap' r)
+| nrec motive z s n => nrec motive⟨r.2.1⟩ (z.rmap' r) (s.rmap' $ r.lift [2, 0]) (n.rmap' r)
+
+theorem blah : Term.rmap' = Term.rmap := by
+  funext r t
+  induction t generalizing r
+  case var n => simp
+  case app t1 t2 ih1 ih2 => simp [ih1, ih2]
+  case tapp t' A ih => simp [ih]
+  case lam A t' ih => simp [ih]
+  case tlam t' ih => simp [ih]
+  case zero => simp
+  case nrec motive z s n ih1 ih2 ih3 => simp [ih1, ih2, ih3]
+  case succ t' ih => simp [ih]
 
 instance : RenMap Term [Term, Ty] where
-  rmap := Term.rmap
+  rmap := Term.rmap'
+
+theorem Term.rmap_var' {x0} (r : RenVec [Term, Ty]) : (var x0)⟨r,⟩ = var (r.1.act (x0)) := rfl
 
 instance : RenMap Term [Term] where
   rmap r := Term.rmap (r.1, Ren.id Ty, .unit)
 
 instance : RenMap Term [Ty] where
   rmap r := Term.rmap (Ren.id Term, r.1, .unit)
+
+instance : SubstMap Ty [Ty] where
+  smap := sorry
 
 @[simp]
 def Term.smap (σ : Subst Term) (τ : Subst Ty) : Term -> Term
@@ -123,10 +143,21 @@ def Term.smap (σ : Subst Term) (τ : Subst Ty) : Term -> Term
 | tapp t A => tapp (t.smap σ τ) A[τ]
 -- Because `Term` has `Ty` variables, we have to increment `Ty` variables in `σ` by 1
 --                       v-------v
-| tlam t => tlam (t.smap σ⟨𝐫1(Ty)⟩ τ.lift)
+| tlam t => tlam (t.smap (σ⟨𝐫1(Ty)⟩) τ.lift)
 | zero => zero
 | succ t => succ (t.smap σ τ)
 | nrec motive z s n => nrec motive[τ] (z.smap σ τ) (s.smap (σ.lift 2) τ) (n.smap σ τ)
+
+@[simp]
+def Term.smap' (σ : SubstVec [Term, Ty]) : Term -> Term
+| var x => σ.1.act x
+| app t1 t2 => app (t1.smap' σ) (t2.smap' σ)
+| lam A t => lam A[σ.2.1] (t.smap' σ)
+| tapp t A => tapp (t.smap' σ) A[σ.2.1]
+| tlam t => tlam (t.smap' $ (σ.1⟨𝐫1(Ty)⟩, σ.2.lift))
+| zero => zero
+| succ t => succ (t.smap' σ)
+| nrec motive z s n => nrec motive[σ.2.1] (z.smap' σ) (s.smap' (σ.1.lift 2, σ.2)) (n.smap' σ)
 
 
 end SystemFWithNat
